Extend bank to multiple accounts
Note: my initial implementation actually had a bug where I was
specifying the offsets in `Acct` in bytes instead of bits (`n*8` instead
of `n*64`), which I eventually caught when I couldn't prove Acct(n)
was in the domain.

In the meantime, with this bug and without an invariant, verification
was extremely painful (the file would take 30-45s to compile, and VSCode
was so slow in getting results it always had errors in the wrong
places).

src/Dafny/examples/bank.i.dfy
@@ -2,8 +2,11 @@ include "../machine/int_encoding.s.dfy"
 include "../util/marshal.i.dfy"
 include "../jrnl/jrnl.s.dfy"
 
-const Acct1: Addr := Addr(513, 0);
-const Acct2: Addr := Addr(513, 8*8);
+function method Acct(n: nat): (a:Addr)
+requires n < 512
+{
+    Addr(513, n*64)
+}
 
 /*
 Demo of bank transfer using axiomatized journal API
@@ -11,10 +14,30 @@ Demo of bank transfer using axiomatized journal API
 class Bank
 {
     ghost const acct_sum: uint64;
-    ghost var acct1: uint64;
-    ghost var acct2: uint64;
+    ghost var accts: seq<uint64>;
 
     var jrnl: Jrnl;
+
+    static predicate acct_val(jrnl: Jrnl, acct: Addr, val: uint64)
+    reads jrnl, jrnl.Repr
+    requires jrnl.Valid()
+    requires acct in jrnl.domain
+    {
+        jrnl.data[acct] == seq_encode([EncUInt64(val)])
+    }
+
+    predicate Valid()
+    reads this, jrnl, jrnl.Repr
+    {
+        && jrnl.Valid()
+        && |accts| == 512
+        && forall n: nat :: n < 512 ==>
+            (var acct := Acct(n);
+             && acct in jrnl.domain
+             && jrnl.size(acct) == 64
+             && acct_val(jrnl, acct, accts[n]))
+        && acct_sum == sum_nat(accts)
+    }
 
     static method encode_acct(x: uint64) returns (bs:seq<byte>)
     ensures seq_encode([EncUInt64(x)]) == bs
@@ -45,59 +68,73 @@ class Bank
     }
 
     constructor()
-    ensures this.Valid()
-    ensures acct1 == 100 && acct2 == 0
+    ensures Valid()
+    ensures forall n: nat:: n < 512 ==> accts[n] == 100
     {
         // BUG: we can't actually use the constant because then Dafny makes the type
         // of the map display expression map<int,int>.
         assert 6 == KindUInt64;
         var kinds: map<Blkno, Kind> := map[513:=6];
         var jrnl := new Jrnl(kinds);
+
+        assert forall n: nat :: n < 512 ==>
+            (var acct := Acct(n);
+             && acct in jrnl.domain
+             && jrnl.size(acct) == 64);
+
         var hundred_acct := encode_acct(100);
-        var zero_acct := encode_acct(0);
-        jrnl.Write(Acct1, hundred_acct);
-        jrnl.Write(Acct2, zero_acct);
+        var n := 0;
+        while n < 512
+        invariant 0 <= n <= 512
+        invariant jrnl.Valid()
+        invariant forall k:: 0 <= k < n ==> acct_val(jrnl, Acct(k), 100)
+        decreases (512-n)
+        {
+            jrnl.Write(Acct(n), hundred_acct);
+            n := n + 1;
+        }
+        assert jrnl.Valid();
+        assert forall n: nat :: n < 512 ==>
+            (var acct := Acct(n);
+             && acct in jrnl.domain
+             && jrnl.size(acct) == 64
+             && acct_val(jrnl, Acct(n), 100));
+
         this.jrnl := jrnl;
 
-        acct1 := 100;
-        acct2 := 0;
-        acct_sum := 100;
-    }
-
-    predicate Valid()
-    reads this, jrnl, jrnl.Repr
-    {
-        && jrnl.Valid()
-        && Acct1 in jrnl.domain
-        && Acct2 in jrnl.domain
-        && jrnl.size(Acct1) == 64
-        && jrnl.size(Acct2) == 64
-        && jrnl.data[Acct1] == seq_encode([EncUInt64(acct1)])
-        && jrnl.data[Acct2] == seq_encode([EncUInt64(acct2)])
-        && acct_sum == acct1 + acct2
+        // NOTE: this was really annoying to figure out - turns out needed the
+        // accounts to be a repeat of nats instead of uint64 (hence the extra
+        // let binding and type annotation)
+        var new_accts: seq<nat> := repeat(100, 512);
+        sum_repeat(100, 512);
+        accts := new_accts;
+        acct_sum := 512*100;
     }
 
     // NOTE: this should be interpreted as the body of a transaction, which
     // needs to be surrounded with code to check for errors and abort
-    method transfer()
+    method transfer(acct1: nat, acct2: nat)
     requires Valid() ensures Valid()
     modifies {this,jrnl}
-    requires 0 < acct1
-    requires acct2+1 < 0x1_0000_0000_0000_000
-    ensures acct1 == old(acct1) - 1
-    ensures acct2 == old(acct2) + 1
+    requires acct1 < 512 && acct2 < 512 && acct1 != acct2
+    requires 0 < accts[acct1]
+    requires accts[acct2] < 0x1_0000_0000_0000_000-1
+    ensures accts == old(accts[acct1:=accts[acct1]-1][acct2:=accts[acct2]+1])
     {
-        var x := jrnl.Read(Acct1, 64);
-        var acct1_val := decode_acct(x.obj, acct1);
+        var x := jrnl.Read(Acct(acct1), 64);
+        var acct1_val := decode_acct(x.obj, accts[acct1]);
         x.obj := encode_acct(acct1_val-1);
         x.SetDirty();
-        acct1 := acct1 - 1;
+        sum_update(accts, acct1, acct1_val-1);
+        accts := accts[acct1:=acct1_val-1];
 
-        x := jrnl.Read(Acct2, 64);
-        var acct2_val := decode_acct(x.obj, acct2);
+        x := jrnl.Read(Acct(acct2), 64);
+        var acct2_val := decode_acct(x.obj, accts[acct2]);
         x.obj := encode_acct(acct2_val+1);
         x.SetDirty();
-        acct2 := acct2 + 1;
+        sum_update(accts, acct2, acct2_val+1);
+        accts := accts[acct2:=acct2_val+1];
+
     }
 
     // this is kind of silly but it gets the point across (without requiring the
@@ -105,7 +142,7 @@ class Bank
     method audit() returns (b:bool)
     modifies {}
     requires Valid()
-    ensures b == (acct1 + acct2 == acct_sum)
+    ensures b == (sum_nat(accts) == acct_sum)
     {
         return true;
     }
