src/Dafny/machine/machine.s.dfy
@@ -1,2 +1,2 @@
 type byte = bv8
-type uint64 = x:int | x < 0x1_0000_0000_0000_0000
+type uint64 = x:int | 0 <= x < 0x1_0000_0000_0000_0000
