src/Dafny/util/collections.dfy
@@ -1,6 +1,6 @@
 // repeat
 
-function method
+function method {:opaque}
 repeat<T>(x: T, count: nat): (xs:seq<T>) decreases count
 ensures |xs| == count && forall i :: 0 <= i < |xs| ==> xs[i] == x
 {
@@ -42,4 +42,34 @@ requires prefix_of(s1, s2)
 requires n <= |s1|
 ensures prefix_of(s1[n..], s2[n..])
 {
+}
+
+// summation
+
+function method sum_nat(xs: seq<nat>): nat
+decreases xs
+{
+    if xs == [] then 0
+    else xs[0] + sum_nat(xs[1..])
+}
+
+lemma {:induction count} sum_repeat(x: nat, count: nat)
+ensures sum_nat(repeat(x, count)) == count * x
+{
+    reveal_repeat();
+}
+
+// NOTE(tej): if you happen to know the proof, then Dafny can automatically
+// prove this with just {:induction xs, i} (but not just i or xs or even i, xs)
+lemma {:induction xs, i} sum_update(xs: seq<nat>, i:nat, x: nat)
+requires i < |xs|
+decreases xs
+ensures sum_nat(xs[i:=x]) == sum_nat(xs)-xs[i]+x
+{
+    assert 0 < |xs|;
+    if i == 0 {}
+    else {
+        // assert (xs[i:=x])[1..] == xs[1..][i-1:=x];
+        sum_update(xs[1..], i-1, x);
+    }
 }
